theories/tree_borrows/steps_retag.v
@@ -23,177 +23,42 @@ Implicit Types f : fname.
 
 (** ** Retags *)
 
-Definition pointer_kind_to_tag_unprotected (pk : pointer_kind) : option tag_kind := match pk with
-  Box im | MutRef im => match im with TyFrz => Some (tk_unq tk_res) | _ => None end (* can not have unprotected IM pointers around *)
-| ShrRef => Some tk_pub end.
-Definition pointer_kind_to_tag_protected (pk : pointer_kind) : tag_kind := match pk with
-  Box _ | MutRef _ => tk_unq tk_res (* for protected, IM is not an issue *)
-| ShrRef => tk_pub end.
+Lemma tree_access_succeeds_heap_value σ b ak tg blk off sz :
+  state_wf σ →
+  trees_contain tg σ.(strs) blk →
+  is_Some (apply_within_trees (memory_access_maybe_nonchildren_only b ak σ.(scs) tg (off, sz)) blk σ.(strs)) →
+  is_Some (read_mem (blk, off) sz σ.(shp)).
+Proof.
+  intros Hwf Hcont [trs' (tr&Htr&(tr'&Htr'&[= <-])%bind_Some)%bind_Some].
+  eapply read_mem_is_Some.
+  intros m Hm.
+  pose proof (state_wf_roots_active _ Hwf _ _ Htr) as Hcompat.
+  destruct tr as [|it tr1 tr2]; first done. simpl in Hcompat.
+  destruct Hcompat as ((Hprot&Hroot)&->).
+  specialize (Hroot (off + m)). rewrite /shift_loc /=.
+  eapply elem_of_dom. destruct (item_lookup it (off + m)) as [[] [| | |]] eqn:Hlookup; simplify_eq; try done.
+  exfalso.
+  rewrite /memory_access_maybe_nonchildren_only /tree_apply_access /= in Htr'.
+  eapply bind_Some in Htr' as (it'&Hit'&_).
+  rewrite /trees_contain /trees_at_block Htr in Hcont.
+  rewrite /item_apply_access in Hit'.
+  eapply bind_Some in Hit' as (perm'&Hperm'&_).
+  rewrite /permissions_apply_range' in Hperm'.
+  unshelve eapply mk_is_Some, mem_apply_range'_success_condition in Hperm' as (pp'&Hpp').
+  1: exact (off + m).
+  2: { rewrite /range'_contains. simpl. lia. }
+  rewrite /item_lookup in Hlookup. rewrite Hlookup in Hpp'. simpl in Hpp'.
+  rewrite /rel_dec /= decide_True in Hpp'; last first.
+  { eapply root_node_IsParentChild. 1: by eapply Hwf. done. }
+  edestruct maybe_non_children_only_effect_or_nop_strong as [(Heq&Hsc)|(Heq&Hb&(ii&Hii))].
+    all: erewrite Heq in Hpp'; clear Heq.
+  2: done. clear Hsc.
+  rewrite /apply_access_perm /apply_access_perm_inner /= in Hpp'.
+  by destruct ak.
+Qed.
 
 (** *** Retags without protectors *)
 
-
-(*
-Lemma bor_interp_retag_default σ_t σ_s c l ot T α' mut :
-  let pk : pointer_kind := RefPtr mut in
-  let pm := match mut with Mutable => Unique | Immutable => SharedReadOnly end in
-  let tk := match mut with Mutable => tk_unq | Immutable => tk_pub end in
-  retag σ_s.(sst) σ_s.(snp) σ_s.(scs) c l ot Default pk T = Some (Tagged σ_s.(snp), α', S σ_s.(snp)) →
-  c ∈ σ_s.(scs) →
-  (if mut is Immutable then is_freeze T else True) →
-  state_wf (mkState σ_t.(shp) α' σ_t.(scs) (S σ_t.(snp)) σ_t.(snc)) →   (* could remove that assumption *)
-  state_wf (mkState σ_s.(shp) α' σ_s.(scs) (S σ_s.(snp)) σ_s.(snc)) →   (* could remove that assumption *)
-  sc_rel (ScPtr l ot) (ScPtr l ot) -∗
-  bor_interp sc_rel σ_t σ_s ==∗ ∃ v_t v_s,
-  ⌜length v_t = tsize T⌝ ∗
-  ⌜length v_s = tsize T⌝ ∗
-  value_rel v_t v_s ∗
-  σ_t.(snp) $$ tk ∗
-  l ↦t∗[tk]{σ_t.(snp)} v_t ∗
-  l ↦s∗[tk]{σ_t.(snp)} v_s ∗
-  match mut with
-  | Mutable => True
-  | Immutable =>
-    sc_rel (ScPtr l (Tagged (σ_t.(snp)))) (ScPtr l (Tagged (σ_t.(snp))))
-  end ∗
-  bor_interp sc_rel (mkState σ_t.(shp) α' σ_t.(scs) (S σ_t.(snp)) σ_t.(snc)) (mkState σ_s.(shp) α' σ_s.(scs) (S σ_s.(snp)) σ_s.(snc)).
-Proof.
-  intros pk pm tk Hretag Hc_in Hfreeze Hwf'_t Hwf'_s.
-  iIntros "Hscrel Hbor". iDestruct "Hbor" as "(%M_call & %M_tag & %M_t & %M_s & (Hc & Htag_auth & Htag_t_auth & Htag_s_auth) & Htainted & Hpub_cid & #Hsrel & %Hcall_interp & %Htag_interp & %Hwf_s & %Hwf_t)".
-
-  iDestruct "Hscrel" as "[_ Hrel]".
-  iAssert (⌜untagged_or_public M_tag ot⌝)%I as %Hpub.
-  { iDestruct "Hrel" as "[[-> _] | (%t1 & %t2 & -> & -> & <- & Hpub)]"; first done.
-    iPoseProof (tkmap_lookup with "Htag_auth Hpub") as "%". done.
-  }
-  pose nt := (snp σ_t).
-
-  have Hin_dom := retag_Some_dom _ _ _ _ _ _ _ pk _ _ _ _ I Hretag.
-  iPoseProof (state_rel_dom_eq with "Hsrel") as "%Hdom_eq".
-  destruct (read_mem_is_Some l (tsize T) σ_s.(shp)) as [v_s Hv_s].
-  { setoid_rewrite (state_wf_dom _ Hwf_s). done. }
-  destruct (read_mem_is_Some l (tsize T) σ_t.(shp)) as [v_t Hv_t].
-  { rewrite Hdom_eq. setoid_rewrite (state_wf_dom _ Hwf_s). done. }
-  destruct (read_mem_values _ _ _ _ Hv_s) as [Hlen_s Hshp_s].
-  destruct (read_mem_values _ _ _ _ Hv_t) as [Hlen_t Hshp_t].
-
-  (* allocate resources *)
-  assert (M_tag !! nt = None) as Htag_none.
-  { destruct (M_tag !! nt) as [[tk' []] | ] eqn:Ht_some; last done.
-    apply Htag_interp in Ht_some as [Hcontra _]. lia. }
-  destruct Htag_interp as (Htag_interp & Ht_dom & Hs_dom).
-  iMod (tkmap_insert tk _ tt Htag_none with "Htag_auth") as "[Htag_auth Hnt]".
-  iMod (ghost_map_array_tag_insert _ _ v_t nt l with "Htag_t_auth") as "[Ht Htag_t_auth]".
-  { intros i Hi. destruct (M_t !! (nt, l +ₗ i)) eqn:Hmt; last done.
-    destruct (Ht_dom nt (l +ₗ i) ltac:(eauto)) as (? & ?); congruence. }
-  iMod (ghost_map_array_tag_insert _ _ v_s nt l with "Htag_s_auth") as "[Hs Htag_s_auth]".
-  { intros i Hi. destruct (M_s !! (nt, l +ₗ i)) eqn:Hmt; last done.
-    destruct (Hs_dom nt (l +ₗ i) ltac:(eauto)) as (? & ?); congruence. }
-  iMod (ghost_map_array_tag_tk _ _ _ _ tk with "Ht") as "Ht".
-  iMod (ghost_map_array_tag_tk _ _ _ _ tk with "Hs") as "Hs".
-  iModIntro.
-  iAssert (nt $$ tk ∗ if tk is tk_pub then nt $$ tk_pub else True)%I  with "[Hnt]" as "[$ Hpubt]".
-  { destruct tk; eauto. }
-  iExists v_t, v_s. iSplit; first done. iSplit; first done. iFrame "Ht Hs".
-
-  iAssert (⌜retag σ_t.(sst) σ_t.(snp) σ_t.(scs) c l ot Default pk T = Some (Tagged nt, α', S (σ_t.(snp)))⌝)%I as "%Hretag_t".
-  { iPoseProof (state_rel_calls_eq with "Hsrel") as "<-".
-    iPoseProof (state_rel_stacks_eq with "Hsrel") as "<-".
-    subst nt. iPoseProof (state_rel_snp_eq with "Hsrel") as "<-". done. }
-  (* proving the value relation *)
-  iAssert (value_rel v_t v_s)%I as "#Hvrel"; last iFrame "Hvrel".
-  { iApply big_sepL2_forall; iSplit; first (iPureIntro;lia).
-    iIntros (i sc_t sc_s) "%Hs_t %Hs_v".
-    assert (i < tsize T)%nat as Hi. { rewrite -Hlen_t. eapply lookup_lt_is_Some_1. eauto. }
-    assert (Hsome_target : is_Some (σ_t.(shp) !! (l +ₗ i))).
-    { rewrite Hshp_t; last done. apply lookup_lt_is_Some_2. by rewrite Hlen_t. }
-    iPoseProof (state_rel_pub_if_not_priv _ _ _ _ _ _ (l +ₗ i) with "[] Hsrel [Hrel]") as "Hpub"; first done.
-    { iPoseProof (state_rel_calls_eq with "Hsrel") as "%Hcall_eq".
-      iPoseProof (state_rel_stacks_eq with "Hsrel") as "%Hstack_eq".
-      iPureIntro. intros t Hpriv.
-      eapply (priv_loc_UB_retag_access_eq σ_s σ_t); eauto; done. }
-    iPoseProof (pub_loc_lookup with "[] Hpub") as "(%sc_t' & %sc_s' & %Hread_both & Hsc_rel)"; first done.
-    enough (sc_t = sc_t' ∧ sc_s = sc_s') by naive_solver.
-    move : Hs_t Hs_v Hread_both (Hshp_s i Hi) (Hshp_t i Hi).
-    by move => -> -> [-> ->] [= ->] [= ->].
-  }
-
-  iSplitL "Hpubt".
-  { destruct mut; first done. iSplitR; first done. iRight.
-    iExists (σ_t.(snp)), (σ_t.(snp)). do 3 (iSplitR; first done). done. }
-
-  (* re-establishing the interpretation *)
-  iExists M_call, (<[ nt := (tk, ()) ]> M_tag), (array_tag_map l nt v_t ∪ M_t), (array_tag_map l nt v_s ∪ M_s).
-  iFrame. iSplitL "Htainted".
-  { (* tainted *) iApply (tag_tainted_interp_retag with "Htainted"); done. }
-  iSplitL.
-  { (* state relation *)
-    rewrite /state_rel. simpl. iDestruct "Hsrel" as "(-> & %Hs_eq & -> & -> & -> & Hsrel)".
-    do 5 (iSplitL; first done). iIntros (l' Hsl').
-    iDestruct ("Hsrel" $! l' with "[//]") as "[Hpub | [%t' %Hpriv]]"; first (iLeft; iApply "Hpub").
-    iRight. iPureIntro. exists t'.
-    destruct Hpriv as (tk' & Hsome_tk' & Ht_l' & Htk'). exists tk'.
-    assert (t' ≠ nt). { intros ->. simplify_eq. }
-    rewrite lookup_insert_ne; last done.
-    split; first done. split; last done.
-    destruct Ht_l' as (sc0 & Ht_l'). exists sc0.
-    rewrite lookup_union_r; first done.
-    destruct (array_tag_map l nt v_t !! (t', l')) as [ a | ] eqn:Harr; last done.
-    specialize (array_tag_map_lookup1 l nt v_t t' l' ltac:(eauto)) as [Heq _]. congruence.
-  }
-  iSplitL.
-  { (* call interpretation. *)
-    iPureIntro. intros c' M' [Hc' HM']%Hcall_interp. split; first done.
-    intros t' S HS. simpl. specialize (HM' t' S HS) as (Ht' & Hprot).
-    split; first lia. intros l' Hl'.
-    specialize (Hprot l' Hl') as (s & pm' & Hs & Hit & Hpm').
-    specialize (retag_item_active_preserving _ _ _ _ _ _ _ _ _ _ _ _ Hretag_t l' s (Tagged t') c' pm' Hs Hc' Hit) as (s' & -> & Hin'). eauto.
-  }
-  iSplitL.
-  { (* tag interpretation. *)
-    iPoseProof (state_rel_get_pure with "Hsrel") as "%Hp".
-    destruct Hp as (Hsst & Hsnp & Hsnc & Hscs).
-    assert (∀l', M_t !! (nt, l') = None) as HMt_nt.
-    { intros l'. destruct (M_t !! (nt, l')) eqn:HM_t; last done.
-      specialize (Ht_dom nt l' ltac:(eauto)) as (? & ?); congruence. }
-    assert (∀l', M_s !! (nt, l') = None) as HMs_nt.
-    { intros l'. destruct (M_s !! (nt, l')) eqn:HM_s; last done.
-      specialize (Hs_dom nt l' ltac:(eauto)) as (? & ?); congruence. }
-    iPureIntro. split_and!.
-    { intros t tk'. rewrite lookup_insert_Some. intros [[<- [= <-]] | [Hneq Hsome_t]].
-      - cbn. split_and!; [lia | lia | | |].
-        + intros l' sc_t Ha%lookup_union_Some_inv_l; last done.
-          specialize (array_tag_map_lookup2 l nt v_t nt l' ltac:(eauto)) as [_ (i & Hi & ->)].
-          eapply loc_controlled_retag_ref; [ done | done |  done | lia | ].
-          move : Ha. rewrite array_tag_map_lookup_Some; last done. move => <-. apply Hshp_t. lia.
-        + intros l' sc_s Ha%lookup_union_Some_inv_l; last done.
-          specialize (array_tag_map_lookup2 l nt v_s nt l' ltac:(eauto)) as [_ (i & Hi & ->)].
-          subst nt. rewrite -Hsnp. eapply loc_controlled_retag_ref; [ done | done | done | lia | ].
-          move : Ha. rewrite array_tag_map_lookup_Some; last done. move => <-. apply Hshp_s. lia.
-        + apply dom_agree_on_tag_union. { apply dom_agree_on_tag_array_tag_map. lia. }
-          apply dom_agree_on_tag_not_elem; done.
-      - cbn.
-        specialize (Htag_interp t tk' Hsome_t) as (Ht_t & Ht_s & Hcontrolled_t & Hcontrolled_s & Hagree).
-        split_and!; [ lia | lia | | | ].
-        + intros l' sc_t Ha. rewrite lookup_union_r in Ha; last by apply array_tag_map_lookup_None.
-          apply Hcontrolled_t in Ha.
-          eapply loc_controlled_retag_update; [done | done | | done | done].
-          intros <-. destruct tk'; [ done | | ]; move : Hsome_t Hpub; congruence.
-        + intros l' sc_s Ha. rewrite lookup_union_r in Ha; last by apply array_tag_map_lookup_None.
-          apply Hcontrolled_s in Ha.
-          eapply loc_controlled_retag_update; [done | done | | done | done].
-          intros <-. destruct tk'; [ done | | ]; move : Hsome_t Hpub; congruence.
-        + apply dom_agree_on_tag_union; last done.
-          apply dom_agree_on_tag_not_elem; apply array_tag_map_lookup_None; done.
-    }
-    { intros t l'.
-      rewrite lookup_union_is_Some lookup_insert_is_Some'. intros [[-> _]%array_tag_map_lookup2 | H%Ht_dom]; eauto. }
-    { intros t l'.
-      rewrite lookup_union_is_Some lookup_insert_is_Some'. intros [[-> _]%array_tag_map_lookup2 | H%Hs_dom]; eauto. }
-  }
-  done.
-Qed.
-*)
 
 Lemma sim_retag_default sz l_t l_s ot c pk tk π Φ :
   pointer_kind_to_tag_unprotected pk = Some tk → (* forbid interior mutability  *)
@@ -217,7 +82,7 @@ Proof.
   odestruct (trees_equal_create_child _ _ _ _ _ _ _ _ _ _ _ _ _ _ _ _ _ _ Hstrs_eq Happly1_s) as (trs1_t&Happly1_t&Hstrs1_eq).
   1,3: eapply Hwf_s. 2: rewrite Hsnc_eq Hsnp_eq. 1,2: eapply Hwf_t. 1: by eapply Hwf_s.
   1-2: done.
-  eapply retag_step_wf_inner in Hwf_s as X. 1: destruct X as (Hwf_mid_s&Hntinmid).
+  eapply retag_step_wf_inner in Hwf_s as X. 1: destruct X as (Hwf_mid_s&Hntinmid_s).
   2-5: done.
   eapply retag_step_wf_inner in Hwf_t as X. 1: destruct X as (Hwf_mid_t&_).
   5: by rewrite Hscs_eq Hsnp_eq in Happly1_t. 4: by rewrite -Hscs_eq. 2-3: setoid_rewrite <- trees_equal_same_tags; last done. 2: done. 2: by rewrite -Hsnp_eq.
@@ -225,7 +90,59 @@ Proof.
   1: exact Hstrs1_eq. 1: apply Hwf_mid_s. 1: apply Hwf_mid_t. 1: done. 1: by eapply mk_is_Some.
   opose proof (trees_equal_preserved_by_access _ _ Hstrs1_eq _ Happly2_s Happly2_t) as Hstrs2_eq.
   1: eapply Hwf_mid_s. 1: eapply Hwf_mid_t. 1: done.
-  clear Hstrs1_eq Hwf_mid_s Hwf_mid_t Hntinmid. (* TODO refactor the above into a separate lemma, maybe? *)
+
+  odestruct (tree_access_succeeds_heap_value _ false) as (v_s&Hv_s).
+  1: apply Hwf_mid_s. 2: eapply mk_is_Some, Happly2_s. 1: done. simpl in Hv_s.
+  odestruct (tree_access_succeeds_heap_value _ false) as (v_t&Hv_t).
+  1: apply Hwf_mid_t. 2: rewrite /= -Hscs_eq; eapply mk_is_Some, Happly2_t. 1: simpl; setoid_rewrite <- trees_equal_same_tags; try done. simpl in Hv_t.
+
+  opose proof (state_wf_tree_unq _ Hwf_mid_t) as Hwf_trs1_t.
+  opose proof (state_wf_tree_unq _ Hwf_mid_s) as Hwf_trs1_s.
+  pose proof Hntinmid_s as Hntinmid_t.
+  setoid_rewrite trees_equal_same_tags in Hntinmid_t. 2: done.
+  clear Hstrs1_eq. (* TODO refactor the above into a separate lemma, maybe? *)
+
+  iDestruct "Hbor" as "(%M_call & %M_tag & %M_t & %M_s & (Hc & Htag_auth & Htag_t_auth & Htag_s_auth) & Hpub_cid & #Hsrel & %Hcall_interp & %Htag_interp & _ & _)".
+  iDestruct (tkmap_lookup with "Htag_auth Hotpub") as "%Hotpub".
+  assert (M_tag !! snp σ_s = None) as Htagfresh.
+  { destruct (M_tag !! σ_s.(snp)) as [[x []]|] eqn:Heq; last done.
+    destruct Htag_interp as (H1&_). specialize (H1 _ _ Heq) as (Hv&_).
+    rewrite /tag_valid in Hv. lia. }
+  iMod (tkmap_insert tk σ_s.(snp) tt with "Htag_auth") as "(Htag_auth&Htk)". 1: done.
+  iDestruct "Hsrel" as "(_&_&_&_&_&Hsrel)".
+  eapply read_mem_values in Hv_s as (Hlen_v_s&Hhpv_v_s).
+  eapply read_mem_values in Hv_t as (Hlen_v_t&Hhpv_v_t). rewrite /shift_loc /= in Hhpv_v_t, Hhpv_v_s.
+  unshelve iSpecialize ("Hsim" $! σ_s.(snp) v_t v_s _ _).
+  1-2: done.
+
+  opose proof* create_then_access_implies_earlier_access_trees as Hvirtual_t.
+  5: exact Happly2_t. 4: exact Happly1_t. 2-3: setoid_rewrite <- trees_equal_same_tags; first done; done. 1: apply Hwf_t.
+
+  iAssert (value_rel v_t v_s)%I as "Hvalrel".
+  { rewrite /value_rel /=. iApply big_sepL2_forall. iSplit; first (iPureIntro; congruence).
+    iIntros (off vt vs Hvt Hvs).
+    ospecialize (Hhpv_v_t off _). 1: rewrite -Hlen_v_t; by eapply lookup_lt_Some.
+    ospecialize (Hhpv_v_s off _). 1: rewrite -Hlen_v_s; by eapply lookup_lt_Some.
+    rewrite Hvt in Hhpv_v_t.
+    iDestruct ("Hsrel" $! _ (mk_is_Some _ _ Hhpv_v_t)) as "[Hpub|(%t&%Hpriv)]".
+    - iDestruct ("Hpub" $! _ Hhpv_v_t) as "(%sc_s&%Hsc_s&Hscrel)".
+      rewrite Hsc_s Hvs in Hhpv_v_s. injection Hhpv_v_s as ->. done.
+    - exfalso. rewrite Hscs_eq in Hvirtual_t.
+      opose proof* priv_loc_access_must_use_same_tag as Heq.
+      5: done. 3-4: done. 1-2: done. all: simpl. 3: exact Hvirtual_t.
+      1: setoid_rewrite <- trees_equal_same_tags; first done; done.
+      1: split; first lia. 1: rewrite -Hlen_v_t. 1: eapply lookup_lt_Some in Hvt; lia.
+      subst t. destruct Hpriv as (tk'&Htk'&[vls Hhl]&[->|(cc&->&Hcc)]). all: congruence. }
+  iSpecialize ("Hsim" with "Hvalrel Htk").
+  assert (M_t !! (snp σ_s, l_s.1) = None) as Hhl_t_None.
+  { destruct Htag_interp as (_&H1&H2&_). destruct (M_t !! (snp σ_s, l_s.1)) eqn:Heq; last done.
+    exfalso. specialize (H1 _ _ (mk_is_Some _ _ Heq)). rewrite Htagfresh in H1. by destruct H1. }
+  iMod (ghost_map_array_tag_insert _ _ v_t σ_s.(snp) l_s tk with "Htag_t_auth") as "(Hpt&Htag_t_auth)"; first done.
+  assert (M_s !! (snp σ_s, l_s.1) = None) as Hhl_s_None.
+  { destruct Htag_interp as (_&H1&H2&_). destruct (M_s !! (snp σ_s, l_s.1)) eqn:Heq; last done.
+    exfalso. specialize (H2 _ _ (mk_is_Some _ _ Heq)). rewrite Htagfresh in H2. by destruct H2. }
+  iMod (ghost_map_array_tag_insert _ _ v_s σ_s.(snp) l_s tk with "Htag_s_auth") as "(Hps&Htag_s_auth)"; first done.
+  iSpecialize ("Hsim" with "Hpt Hps").
 
   iModIntro. iSplit.
   { iPureIntro. do 3 eexists. econstructor; econstructor.
@@ -235,19 +152,104 @@ Proof.
   destruct (head_retag_inv _ _ _ _ _ _ _ _ _ _ _ Hhead_t) as (trsX1&trsX2&->&->&Hσ_t'&Hcin_t&Hotin_t&Hntnin_t&HX1&HX2).
   assert (trsX1 = trs1_t) as -> by congruence. clear HX1.
   assert (trsX2 = trs2_t) as -> by congruence. clear HX2.
+
   iModIntro. iExists _, _, _. iSplit.
   { iPureIntro. simpl. econstructor; econstructor. all: done. }
 
-  iDestruct "Hbor" as "(%M_call & %M_tag & %M_t & %M_s & (Hc & Htag_auth & Htag_t_auth & Htag_s_auth) & Hpub_cid & #Hsrel & %Hcall_interp & %Htag_interp & _ & _)".
-  iFrame "HP_t HP_s".
-  (*
-  iDestruct 
-
-
-  rewrite -Hsnp_eq.
-  iFrame "HP_t HP_s". iSplitR "Hsim"; last first.
-  { iSplit; last done. iApply "Hsim". *)
-Admitted.
+  iFrame "HP_t HP_s". rewrite -Hsnp_eq. iFrame "Hsim". simpl.
+  iSplit; last done.
+  iExists _, _, _, _. rewrite /bor_interp_inner. iFrame "Htag_auth Htag_t_auth Htag_s_auth Hc". simpl.
+  iSplit; last iSplit; last iSplit; last iSplit; last iSplit.
+  - iApply pub_cid_interp_preserve_sub. 5: iFrame.
+    1,3: by subst σ_t'. all: done.
+  - subst σ_t'. rewrite -Hsnp_eq. do 5 (iSplit; first done). simpl.
+    iIntros (l Hl). iDestruct ("Hsrel" $! l Hl) as "[Hpub|(%t&%Hpriv)]".
+    + iLeft. iApply "Hpub".
+    + iRight. iExists t. iPureIntro. destruct Hpriv as (tk'&Htk'&Hhl&Htag).
+      exists tk'. split. 1: rewrite lookup_insert_ne //. 1: intros <-; congruence.
+      split. 1: rewrite /heaplet_lookup /= -?insert_union_singleton_l in Hhl|-*; rewrite lookup_insert_ne //; congruence.
+      apply Htag.
+  - iPureIntro. subst σ_t'. intros cc M' HM'. specialize (Hcall_interp cc M' HM') as (Hc1&Hc2). simpl.
+    split; first done. intros tt L HL. specialize (Hc2 tt L HL) as (Hc3&Hc4).
+    split. 1: eapply tag_valid_mono; first done; lia.
+    intros l ps Hps. specialize (Hc4 l ps Hps).
+    eapply (tag_protected_preserved_by_create ps ot (snp σ_s) pk Default (scs σ_s)) in Hc4.
+    4: exact Happly1_t. 2: eapply Hwf_t. 2: { intros <-. rewrite /tag_valid in Hc3. lia. }
+    eapply tag_protected_preserved_by_access.
+    2: exact Happly2_t. 2: rewrite Hscs_eq; apply Hc1. 2: done. 1: eapply Hwf_trs1_t.
+  - iPureIntro. destruct Htag_interp as (Ht1&Ht2&Ht3&Ht4&Ht5).
+    split_and!.
+    2-5: rewrite /array_tag_map -!insert_union_singleton_l.
+    2-3: intros t blk (x & [([= <- <-]&<-)|(?&?)]%lookup_insert_Some);
+         [by rewrite lookup_insert|eapply lookup_insert_is_Some'; right].
+         2: eapply Ht2. 3: eapply Ht3. 2-3: by eapply mk_is_Some.
+    2,3: intros tg l1 l2; rewrite !dom_insert_L;
+         intros [[= Heq1 Heq2]%elem_of_singleton|H1%elem_of_dom]%elem_of_union;
+         intros [[= Heq3 Heq4]%elem_of_singleton|H2%elem_of_dom]%elem_of_union; simplify_eq;
+         [done|rename H2 into H1| | ].
+         4: eapply Ht4; by eapply elem_of_dom.
+         6: eapply Ht5; by eapply elem_of_dom.
+         2,3: eapply Ht2 in H1. 4,5: eapply Ht3 in H1.
+         2-5: rewrite Htagfresh in H1; by destruct H1.
+    intros t tk' [(<-&[= <-])|(Hne&Hin)]%lookup_insert_Some; last first.
+    + subst σ_t'. specialize (Ht1 _ _ Hin) as (Htt1&Htt2&Htt3&Htt4&Htt5).
+      split_and!.
+      1-2: simpl; eapply tag_valid_mono; last reflexivity.
+      1,3: done. 1,2: lia.
+      all: rewrite /array_tag_map -!insert_union_singleton_l.
+      3: { eapply dom_agree_on_tag_upd_ne; last exact Htt5.
+           intros <-. rewrite /tag_valid in Htt1; lia. }
+      1-2: intros l sc (Mhl&H1%lookup_insert_Some&H2)%bind_Some;
+           simpl in H1; destruct H1 as [([= Hl1]&<-)|(Hnel&Hlu)].
+      1,3: subst t; rewrite /tag_valid in Htt2,Htt3; lia.
+      * ospecialize (Htt3 l sc _).
+        1: rewrite /heaplet_lookup Hlu /= H2 //.
+        eapply loc_controlled_read_preserved_everywhere. 4: exact Hwf_mid_t. all: simpl. 2-3: done.
+        1: rewrite -Hscs_eq; done. 1: done.
+        eapply loc_controlled_create_child_preserved_everywhere. 5: exact Hwf_mid_t. 4: exact Hwf_t. all: simpl.
+        1: rewrite Hscs_eq Hsnp_eq in Happly1_t; done. 1-2: done. 1-2: done.
+        1: intros ->; rewrite /tag_valid in Htt1,Htt2; lia.
+        1: intros ->; congruence. done.
+      * ospecialize (Htt4 l sc _).
+        1: rewrite /heaplet_lookup Hlu /= H2 //.
+        eapply loc_controlled_read_preserved_everywhere. 4: exact Hwf_mid_s. all: simpl. 2-3: done.
+        1: done. 1: done.
+        eapply loc_controlled_create_child_preserved_everywhere. 5: exact Hwf_mid_s. 4: exact Hwf_s. all: simpl.
+        1: done. 1-2: done. 1-2: done.
+        1: intros ->; rewrite /tag_valid in Htt1,Htt2; lia.
+        1: intros ->; congruence. done.
+    + subst σ_t'; simpl. split_and!.
+      1-2: rewrite !Hsnp_eq /tag_valid; lia.
+      all: rewrite /array_tag_map -!insert_union_singleton_l /=.
+      3: { eapply dom_agree_on_tag_update_same. 2: eapply list_to_heaplet_dom_1; congruence.
+           split; intros l [x (M&HM%mk_is_Some&HHM)%bind_Some]; simpl in HM.
+           1: eapply Ht2 in HM. 2: eapply Ht3 in HM.
+           all: rewrite Htagfresh in HM; by destruct HM. }
+       1-2: intros l sc (Mhl&H1%lookup_insert_Some&H2)%bind_Some;
+            simpl in H1; destruct H1 as [([= Hl1]&<-)|(Hne&Hlu)].
+       * simpl in H2. eapply list_to_heaplet_lookup_Some in H2 as H2'.
+         assert (∃ (i:nat), l.2 = l_s.2 + i) as (off&Hoff). 1: exists (Z.to_nat (l.2 - l_s.2)); lia.
+         rewrite Hoff list_to_heaplet_nth -Hhpv_v_t in H2. 2: lia.
+         rewrite -Hoff in H2. eapply loc_controlled_read_after_reborrow_creates.
+         1: exact Happly1_t. 1: exact Happly2_t. 1-4,8: done.
+         1: by rewrite Hsnp_eq. 2: lia. 1: destruct l as [l1 l2]; simpl in *; subst l1; done.
+       * eapply mk_is_Some, Ht2 in Hlu. rewrite Htagfresh in Hlu. by destruct Hlu.
+       * simpl in H2. eapply list_to_heaplet_lookup_Some in H2 as H2'.
+         assert (∃ (i:nat), l.2 = l_s.2 + i) as (off&Hoff). 1: exists (Z.to_nat (l.2 - l_s.2)); lia.
+         rewrite Hoff list_to_heaplet_nth -Hhpv_v_s in H2. 2: lia.
+         rewrite -Hoff in H2. eapply loc_controlled_read_after_reborrow_creates.
+         1: exact Happly1_s. 1: exact Happly2_s. 1-5,8: done.
+         2: lia. 1: destruct l as [l1 l2]; simpl in *; subst l1; done.
+       * eapply mk_is_Some, Ht3 in Hlu. rewrite Htagfresh in Hlu. by destruct Hlu.
+  - (* source state wf *)
+    iPureIntro. eapply retag_step_wf_inner in Hwf_s as (Hwf_s&Hccc). 2-5: done.
+    eapply read_step_wf_inner in Hwf_s; done.
+  - (* target state wf *)
+    iPureIntro. subst σ_t'. eapply retag_step_wf_inner in Hwf_t as (Hwf_t&Hccc). 2-5: try done.
+    2: by rewrite -Hscs_eq -Hsnp_eq. simpl in Hwf_t.
+    eapply read_step_wf_inner in Hwf_t. 1: done. all: simpl.
+    2: by rewrite -Hscs_eq. by rewrite Hsnp_eq.
+Qed.
 (*
 
 (** *** Retags with protectors *)
